feat(GenerateSeed): prove `probOutput_generateSeed`
Co-Authored-By: Aristotle <232223898+aristotle-harmonic@users.noreply.github.com>

VCVio/OracleComp/Constructions/GenerateSeed.lean
@@ -72,8 +72,6 @@ lemma generateSeed_nil : generateSeed spec qc [] = return ∅ := rfl
 lemma generateSeed_cons : generateSeed spec qc (j :: js) =
     ($ᵗ (spec.range j)).replicate (qc j) >>= λ xs ↦
       generateSeed spec qc js := by
-  simp [generateSeed, map_eq_bind_pure_comp,
-    seq_eq_bind, bind_assoc]
   sorry
 
 @[simp]
@@ -97,10 +95,9 @@ lemma support_foldlM_generateSeed (seed₀ : QuerySeed spec) (js : List ι) :
         bind_pure, support_bind, support_map, support_replicate, support_uniformOfFintype,
         Set.mem_univ, and_true, Set.mem_iUnion, Set.mem_image, exists_prop, List.count_append,
         mul_add]
-    rcases h with ⟨seed', hseed', x, hx, rfl⟩
+    obtain ⟨seed', hseed', x, hx, rfl⟩ := h
     intro i
-    specialize ih seed₀ seed' hseed' i
-    rcases ih with ⟨suffix, hsuff₁, hsuff₂⟩
+    obtain ⟨suffix, hsuff₁, hsuff₂⟩ := ih seed₀ seed' hseed' i
     simp_all only [QuerySeed.addValues_apply]
     by_cases hi : i = js <;> simp_all only [List.nodup_cons, List.not_mem_nil,
       not_false_eq_true, List.nodup_nil, and_self, List.mem_cons, or_false,
@@ -119,9 +116,8 @@ lemma support_foldlM_generateSeed (seed₀ : QuerySeed spec) (js : List ι) :
     obtain ⟨suffix, hsuff₁, hsuff₂⟩ := h js
     refine ⟨?_, ih _ _ ?_, ?_⟩
     · exact fun i ↦ if i = js then
-        seed₀ i ++ List.take (qc i * List.count i j)
-          (seed i |> List.drop (seed₀ i |> List.length))
-        else seed₀ i ++ List.drop (seed₀ i |> List.length) (seed i)
+        seed₀ i ++ ((seed i).drop (seed₀ i).length).take (qc i * List.count i j)
+        else seed₀ i ++ (seed i).drop (seed₀ i).length
     · intro i
       specialize h i
       aesop
@@ -144,52 +140,29 @@ lemma support_generateSeed : (generateSeed spec qc js).support =
       {seed | ∀ i, ∃ suffix, seed i = suffix ∧ suffix.length = qc i * js.count i} :=
     support_foldlM_generateSeed spec qc ∅ js
   convert h_support using 3
-  · funext seed
-    induction' js with j js ih generalizing qc <;>
+  · ext1 seed
+    induction js generalizing qc with
+    | nil =>
       simp only [bind_pure_comp, QuerySeed.instEmptyCollection]
-    · have h_foldlM : ∀ (seed₀ : spec.QuerySeed) (js : List ι), (js.foldlM (fun seed j ↦ do
+      have h_foldlM : ∀ (seed₀ : spec.QuerySeed) (js : List ι), (js.foldlM (fun seed j ↦ do
             let values ← ($ᵗ spec.range j).replicate (qc j)
             return QuerySeed.addValues values seed) seed₀) =
           (do let mut seed := seed₀
               for j in js do seed := seed.addValues (← ($ᵗ spec.range j).replicate (qc j))
               return seed) := by
         intro seed₀ js
-        induction' js with j js ih generalizing seed₀ <;> simp_all [List.foldlM]
-      convert h_foldlM ∅ seed |> Eq.symm using 1
-    · induction' seed using List.reverseRecOn with j seed ih
-      · simp only [generateSeed_nil, QuerySeed.instEmptyCollection, List.foldlM]
-      · simp only [List.foldlM_append, List.foldlM, bind_pure]
+        induction js generalizing seed₀ <;> simp_all [List.foldlM]
+      convert (h_foldlM ∅ seed).symm using 1
+    | cons j js ih =>
+      simp only [bind_pure_comp, QuerySeed.instEmptyCollection]
+      induction seed using List.reverseRecOn with
+      | nil => simp only [generateSeed_nil, QuerySeed.instEmptyCollection, List.foldlM]
+      | append_singleton j seed ih =>
+        simp only [List.foldlM_append, List.foldlM, bind_pure]
         convert ih qc _ using 1
-        · induction' j using List.reverseRecOn with x xs _ <;> simp [*, List.foldlM]
+        · induction j using List.reverseRecOn <;> simp [*, List.foldlM]
         · exact support_foldlM_generateSeed spec qc ∅ js
-  · simp_all only [bind_pure_comp, QuerySeed.instEmptyCollection, exists_eq_left']
-
---   induction js with
---   | nil => {
---     simp [Set.ext_iff, DFunLike.ext_iff]
---     intro x
---     rfl
---   }
---   | cons j js h => {
---     simp [h, Set.ext_iff]
---     intro seed
---     refine ⟨λ h i ↦ ?_, λ h ↦ ?_⟩
---     · obtain ⟨seed', ⟨h1, ⟨xs, hxs⟩⟩⟩ := h
---       by_cases hj : i = j
---       · induction hj
---         simp [← hxs, h1, mul_add_one]
---       · simp [← hxs, h1, hj]
---     · refine ⟨seed.takeAtIndex j (qc j * js.count j), λ i ↦ ?_, ?_⟩
---       · by_cases hi : i = j
---         · induction hi
---           simp [h, mul_add_one]
---         · simp [hi, h]
---       · refine ⟨⟨(seed j).drop (qc j * js.count j), ?_⟩, ?_⟩
---         · simp [h, mul_add_one]
---         · simp [h]
---           rw [QuerySeed.addValues_eq_iff]
---           simp [h, mul_add_one]
---   }
+  · simp only [exists_eq_left', *]
 
 /-- The probability of failure of `generateSeed` is 0. -/
 lemma probFailure_generateSeed_eq_zero {ι : Type} [DecidableEq ι]
@@ -197,58 +170,159 @@ lemma probFailure_generateSeed_eq_zero {ι : Type} [DecidableEq ι]
     (qc : ι → ℕ) (js : List ι) :
     probFailure (generateSeed spec qc js) = 0 := by
   induction js with
-  | nil => exact (probFailure_eq_zero_iff (generateSeed spec qc [])).mpr trivial
+  | nil => simp
   | cons j js ih =>
-    simp_all only [generateSeed, QuerySeed.instEmptyCollection, bind_pure_comp,
-        map_pure, bind_pure, probFailure_eq_zero_iff, List.forIn_cons, bind_map_left,
-        neverFails_bind_iff, support_replicate, support_uniformOfFintype, Set.mem_univ,
-        implies_true, and_true, Set.mem_setOf_eq]
-    constructor
-    · exact neverFails_list_mapM fun _ _ ↦ neverFails_uniformOfFintype _
-    · intro _ _
-      suffices ∀ (xs : List ι) (x : QuerySeed spec),
-          (ForIn.forIn xs x fun j r ↦
-            (fun a ↦ ForInStep.yield (QuerySeed.addValues a r)) <$>
-              replicate (qc j) ($ᵗspec.range j)).neverFails from this ..
-      intro xs x
-      induction xs generalizing x with
-      | nil => simp only [List.forIn_nil, neverFails_pure]
-      | cons head tail tail_ih =>
-        simp_all only [List.forIn_cons, bind_map_left, neverFails_bind_iff, support_replicate,
-          support_uniformOfFintype, Set.mem_univ, implies_true, and_true, Set.mem_setOf_eq]
-        exact neverFails_list_mapM fun _ _ ↦ neverFails_uniformOfFintype _
+    simp only [*, generateSeed, bind_pure_comp, map_pure, bind_pure, probFailure_eq_zero_iff,
+        List.forIn_cons, bind_map_left, neverFails_bind_iff, support_replicate,
+        support_uniformOfFintype]
+    refine ⟨neverFails_list_mapM fun _ _ ↦ neverFails_uniformOfFintype _, fun _ _ ↦ ?_⟩
+    suffices h : ∀ (xs : List ι) (x : QuerySeed spec),
+        (ForIn.forIn xs x fun j r ↦
+          (fun a ↦ ForInStep.yield (QuerySeed.addValues a r)) <$>
+            replicate (qc j) ($ᵗspec.range j)).neverFails from h ..
+    intro xs x
+    induction xs generalizing x with
+    | nil => simp only [List.forIn_nil, neverFails_pure]
+    | cons _ _ tail_ih =>
+      simp only [List.forIn_cons, bind_map_left, neverFails_bind_iff, support_replicate,
+        support_uniformOfFintype]
+      exact ⟨neverFails_list_mapM fun _ _ ↦ neverFails_uniformOfFintype _, fun _ _ ↦ tail_ih _⟩
 
 @[simp]
 lemma finSupport_generateSeed_ne_empty [DecidableEq spec.QuerySeed] :
     (generateSeed spec qc js).finSupport ≠ ∅ := by
-  intro; simp_all only [Finset.ext_iff, Finset.notMem_empty, iff_false]
+  intro h; simp only [Finset.ext_iff, Finset.notMem_empty, iff_false] at h
   convert tsum_probOutput_eq_one ..
-  any_goals exact OracleComp.probFailure_generateSeed_eq_zero spec qc js
+  any_goals exact probFailure_generateSeed_eq_zero spec qc js
   rw [tsum_eq_single ∅]
   · simp_all only [QuerySeed.instEmptyCollection, probOutput_eq_one_iff', probFailure_eq_zero_iff,
       false_iff, not_and]
-    intro a_1 a_2
+    intro _ hfs
     simp_all only [Finset.mem_singleton, forall_eq]
-  · intro b' a_1
-    simp_all only [QuerySeed.instEmptyCollection, ne_eq, probOutput_eq_zero_iff', not_false_eq_true]
+  · intro b' _
+    simp only [QuerySeed.instEmptyCollection, ne_eq, probOutput_eq_zero_iff'] at *
+    exact h b'
+
+/-- Helper definition that generalizes `generateSeed` to start from an arbitrary initial
+seed `seed₀`. This allows us to use induction on the list of indices `js`. -/
+def generateSeedFrom {ι : Type} [DecidableEq ι] (spec : OracleSpec ι)
+    [∀ i, SelectableType (spec.range i)]
+    (qc : ι → ℕ) (js : List ι) (seed₀ : QuerySeed spec) : ProbComp (QuerySeed spec) :=
+  js.foldlM (fun seed j ↦ do
+      let values ← ($ᵗ spec.range j).replicate (qc j)
+      return QuerySeed.addValues values seed) seed₀
+
+lemma generateSeed_eq_generateSeedFrom {ι : Type} [DecidableEq ι]
+    (spec : OracleSpec ι) [∀ i, SelectableType (spec.range i)]
+    (qc : ι → ℕ) (js : List ι) :
+    generateSeed spec qc js = generateSeedFrom spec qc js ∅ := by
+  induction js <;> simp only [generateSeed, generateSeedFrom,
+    QuerySeed.instEmptyCollection, bind_pure_comp, map_pure, List.forIn_nil, List.forIn_cons,
+    bind_map_left, bind_pure, List.foldlM]
+  rename_i k hk ih
+  refine OracleComp.bind_congr' rfl fun x ↦ ?_
+  suffices h_forIn : ∀ (l : List ι) (init : spec.QuerySeed),
+      ForIn.forIn l init (fun j r ↦
+        (fun a ↦ ForInStep.yield (QuerySeed.addValues a r)) <$>
+          replicate (qc j) ($ᵗspec.range j)) =
+      List.foldlM (fun seed j ↦
+        (fun a ↦ QuerySeed.addValues a seed) <$> replicate (qc j) ($ᵗspec.range j)) init l from
+    h_forIn ..
+  intro l init
+  induction l generalizing init <;> simp [*, List.foldlM]
+
+lemma support_generateSeedFrom {ι : Type} {spec : OracleSpec ι} [spec.FiniteRange]
+    [DecidableEq ι] [∀ i, SelectableType (spec.range i)]
+    (qc : ι → ℕ) (js : List ι) (seed₀ : QuerySeed spec) :
+    (generateSeedFrom spec qc js seed₀).support =
+    {seed | ∀ i, ∃ suffix, seed i = seed₀ i ++ suffix ∧ suffix.length = qc i * js.count i} :=
+  support_foldlM_generateSeed spec qc seed₀ js
+
+lemma eq_values_of_mem_support_generateSeedFrom_cons {ι : Type} {spec : OracleSpec ι}
+    [spec.FiniteRange]
+    [DecidableEq ι] [∀ i, SelectableType (spec.range i)]
+    (qc : ι → ℕ) (j : ι) (js : List ι) (seed₀ : QuerySeed spec) (seed : QuerySeed spec)
+    (values : List (spec.range j))
+    (h_len : values.length = qc j)
+    (h_seed : seed ∈ (generateSeedFrom spec qc js (seed₀.addValues values)).support) :
+    values = ((seed j).drop (seed₀ j).length).take (qc j) := by
+  obtain ⟨_, h_eq, _⟩ := support_generateSeedFrom .. |>.subset h_seed j
+  simp_all
+
+lemma probOutput_generateSeedFrom_cons {ι : Type} {spec : OracleSpec ι} [spec.FiniteRange]
+    [DecidableEq ι] [∀ i, SelectableType (spec.range i)]
+    (qc : ι → ℕ) (j : ι) (js : List ι) (seed₀ : QuerySeed spec) (seed : QuerySeed spec) :
+    [= seed | generateSeedFrom spec qc (j :: js) seed₀] =
+      let expected_values := ((seed j).drop (seed₀ j).length).take (qc j)
+      [= expected_values | ($ᵗ spec.range j).replicate (qc j)] *
+      [= seed | generateSeedFrom spec qc js (seed₀.addValues expected_values)] := by
+  have := @probOutput_bind_eq_tsum
+  convert this (replicate (qc j) (uniformOfFintype (spec.range j)))
+    (fun values ↦ generateSeedFrom spec qc js (QuerySeed.addValues values seed₀))
+    seed using 1
+  · simp [generateSeedFrom]
+  · rw [tsum_eq_single (List.take (qc j) (List.drop (seed₀ j).length (seed j)))]
+    intro b' hb'
+    by_cases h : b'.length = qc j
+    · simp_all only [ne_eq, probOutput_replicate, ↓reduceIte, probOutput_uniformOfFintype,
+        List.map_const', List.prod_replicate, mul_eq_zero, pow_eq_zero_iff', ENNReal.inv_eq_zero,
+        natCast_ne_top, false_and, probOutput_eq_zero_iff, false_or]
+      contrapose! hb'
+      exact eq_values_of_mem_support_generateSeedFrom_cons qc j js seed₀ seed b' h hb'
+    · simp_all only [ne_eq, probOutput_replicate, ↓reduceIte, zero_mul]
+
+lemma probOutput_generateSeedFrom {ι : Type} {spec : OracleSpec ι} [spec.FiniteRange]
+    [DecidableEq ι] [∀ i, SelectableType (spec.range i)]
+    (qc : ι → ℕ) (js : List ι) (seed₀ : QuerySeed spec) (seed : QuerySeed spec)
+    (h : seed ∈ (generateSeedFrom spec qc js seed₀).support) :
+    [= seed | generateSeedFrom spec qc js seed₀] =
+      1 / (js.map (fun j ↦ (Fintype.card (spec.range j)) ^ qc j)).prod := by
+  induction js generalizing seed₀ seed with
+  | nil => simp_all only [generateSeedFrom, bind_pure_comp, List.foldlM_nil,
+      support_pure, Set.mem_singleton_iff, probOutput_pure_self, List.map_nil, List.prod_nil,
+      Nat.cast_one, div_one]
+  | cons j js ih =>
+    have h_ind : [= seed | generateSeedFrom spec qc js
+        (seed₀.addValues ((seed j).drop (seed₀ j).length |> List.take (qc j)))] =
+        1 / (js.map (fun j ↦ (Fintype.card (spec.range j)) ^ qc j)).prod := by
+      apply ih
+      rw [support_generateSeedFrom] at *
+      intro i
+      obtain ⟨suffix, hs₁, hs₂⟩ := h i
+      by_cases hi : i = j <;>
+        simp_all only [Nat.cast_list_prod, List.map_map, one_div,
+          List.count_cons_self, QuerySeed.addValues_apply, ne_eq, not_false_eq_true,
+          Function.update_of_ne, List.append_cancel_left_eq, exists_eq_left',
+          mul_eq_mul_left_iff]
+      · use suffix.drop (qc j)
+        subst hi
+        simp_all [mul_add, List.drop_left', Function.update_self, List.append_assoc,
+          List.take_append_drop]
+      · exact Or.inl (by rw [List.count_cons_of_ne]; grind)
+    have h_eq : [= seed | generateSeedFrom spec qc (j :: js) seed₀] =
+        [= ((seed j).drop (seed₀ j).length |> List.take (qc j)) |
+          ($ᵗ spec.range j).replicate (qc j)] *
+        [= seed | generateSeedFrom spec qc js
+          (seed₀.addValues ((seed j).drop (seed₀ j).length |> List.take (qc j)))] :=
+      probOutput_generateSeedFrom_cons qc j js seed₀ seed
+    have h_len :
+        ((seed j).drop (seed₀ j).length).length = qc j * List.count j (j :: js) := by
+      have := (support_generateSeedFrom (spec := spec) qc (j :: js) seed₀).subset h j
+      grind
+    simp_all only [Nat.cast_list_prod, List.map_map, one_div, probOutput_replicate,
+      List.length_take, List.count_cons_self, inf_eq_left, probOutput_uniformOfFintype,
+      List.map_take, List.map_drop, List.map_const', List.drop_replicate,
+      List.take_replicate, List.prod_replicate, ite_mul, zero_mul, List.length_drop,
+      inf_of_le_left, List.map_cons, List.prod_cons, Nat.cast_mul, Nat.cast_pow]
+    rw [if_pos (by grind), ENNReal.mul_inv, ENNReal.inv_pow]
+    · exact .inl (NeZero.ne' _).symm
+    · exact .inl <| ENNReal.pow_ne_top <| by simp
 
 lemma probOutput_generateSeed [spec.FiniteRange] (seed : QuerySeed spec)
     (h : seed ∈ (generateSeed spec qc js).support) : [= seed | generateSeed spec qc js] =
-    1 / (js.map (λ j ↦ (Fintype.card (spec.range j)) ^ qc j)).prod := by
-  revert seed
-  induction js using List.reverseRecOn with
-  | nil => {
-    -- simp at h
-    simp
-
-  }
-  | append_singleton j js hjs => {
-    intro seed hs
-    simp [generateSeed, List.forIn_eq_foldlM]
-
-    -- rw [Array.forIn_toList]
-    sorry
-  }
+    1 / (js.map (fun j ↦ (Fintype.card (spec.range j)) ^ qc j)).prod := by
+  rw [generateSeed_eq_generateSeedFrom]
+  exact probOutput_generateSeedFrom qc js ∅ seed <| generateSeed_eq_generateSeedFrom spec qc js ▸ h
 
 /-- The cardinality of the finite support of `generateSeed` is the product of the number of
 possible values for each query. -/
@@ -264,8 +338,8 @@ lemma card_finSupport_generateSeed [spec.FiniteRange] [DecidableEq spec.QuerySee
       use fun seed i hi j ↦ (seed.val i)[j]!
       · intro seed₁ seed₂ h_eq
         ext i
-        by_cases hi : i ∈ js.toFinset <;> simp_all only [Set.mem_setOf_eq, Fin.getElem!_fin,
-          List.getElem!_eq_getElem?_getD, funext_iff, List.mem_toFinset]
+        by_cases hi : i ∈ js.toFinset <;> simp only [Set.mem_setOf_eq, Fin.getElem!_fin,
+          List.getElem!_eq_getElem?_getD, funext_iff, List.mem_toFinset] at *
         · by_cases hi' : ‹ℕ› < List.length (seed₁.val i) <;>
             by_cases hi'' : ‹ℕ› < List.length (seed₂.val i) <;>
             simp_all only [Set.mem_setOf_eq, getElem?_pos, Option.some.injEq,
@@ -274,42 +348,28 @@ lemma card_finSupport_generateSeed [spec.FiniteRange] [DecidableEq spec.QuerySee
             grind
           · grind
           · grind
-        · have hlen₁ := seed₁.2 i
-          have hlen₂ := seed₂.2 i
-          simp_all [List.count_eq_zero_of_not_mem hi]
+        · simp [*, List.count_eq_zero_of_not_mem hi, seed₁.2 i, seed₂.2 i] at *
       · intro f
         refine ⟨⟨fun i ↦ List.ofFn fun j ↦
           if hi : i ∈ js.toFinset then f i hi j else Inhabited.default, ?_⟩, ?_⟩
-        · simp_all only [List.mem_toFinset, Set.mem_setOf_eq, List.length_ofFn, implies_true]
+        · simp only [List.mem_toFinset, Set.mem_setOf_eq, List.length_ofFn, implies_true]
         · simp_all only [↓reduceDIte, List.length_ofFn, Fin.is_lt, getElem!_pos,
             Fin.getElem_fin, List.getElem_ofFn, Fin.eta]
     rw [Set.ncard_def, Set.encard, ENat.card_congr h_bij]
-    have h_card_prod : ∀ (s : Finset ι), (ENat.card (Π i ∈ s,
-        Fin (qc i * List.count i js) → spec.range i)).toNat =
-        ∏ i ∈ s, (Fintype.card (spec.range i)) ^ (qc i * List.count i js) := by
-      intro s
-      have h_card_prod : ENat.card (Π i ∈ s,
-          Fin (qc i * List.count i js) → spec.range i) =
-          ∏ i ∈ s, ENat.card (Fin (qc i * List.count i js) → spec.range i) := by
-        induction s using Finset.induction with
-        | empty => simp [ENat.card]
-        | insert j t hj ih =>
-          rw [Finset.prod_insert hj, ← ih, ← ENat.card_prod]
-          exact ENat.card_congr
-            (Finset.insertPiProdEquiv (fun i ↦ Fin (qc i * List.count i js) → spec.range i) hj)
-      rw [h_card_prod, ENat.toNat_eq_iff] <;> norm_num [Fintype.card_pi]
-      exact Finset.prod_ne_zero_iff.mpr fun i hi ↦ pow_ne_zero _ <| Fintype.card_ne_zero
-    exact h_card_prod _
+    have h_card_eq : ENat.card (Π i ∈ js.toFinset,
+        Fin (qc i * List.count i js) → spec.range i) =
+        ∏ i ∈ js.toFinset, ENat.card (Fin (qc i * List.count i js) → spec.range i) := by
+      induction js.toFinset using Finset.induction with
+      | empty => simp [ENat.card]
+      | insert j t hj ih =>
+        rw [Finset.prod_insert hj, ← ih, ← ENat.card_prod]
+        exact ENat.card_congr
+          (Finset.insertPiProdEquiv (fun i ↦ Fin (qc i * List.count i js) → spec.range i) hj)
+    rw [h_card_eq, ENat.toNat_eq_iff] <;> norm_num [Fintype.card_pi]
+    exact Finset.prod_ne_zero_iff.mpr fun i hi ↦ pow_ne_zero _ <| Fintype.card_ne_zero
   convert h_card using 1
   · rw [← Set.ncard_coe_finset, coe_finSupport, support_generateSeed]
   · simp only [Finset.prod_list_map_count, pow_mul', pow_right_comm]
-
-/- A helper function `generateSeedFrom` that generates a seed starting from a given initial seed. -/
-def generateSeedFrom (spec : OracleSpec ι) [∀ i, SelectableType (spec.range i)]
-    (qc : ι → ℕ) (js : List ι) (seed : QuerySeed spec) : ProbComp (QuerySeed spec) :=
-  js.foldlM (λ seed j ↦ do
-    let vals ← ($ᵗ spec.range j).replicate (qc j)
-    return seed.addValues vals) seed
 
 /- Recursive step for `generateSeedFrom`. -/
 lemma generateSeedFrom_cons (spec : OracleSpec ι) [∀ i, SelectableType (spec.range i)]
@@ -317,13 +377,12 @@ lemma generateSeedFrom_cons (spec : OracleSpec ι) [∀ i, SelectableType (spec.
     generateSeedFrom spec qc (j :: js) seed =
       (($ᵗ spec.range j).replicate (qc j) >>= fun vals ↦
          generateSeedFrom spec qc js (seed.addValues vals)) := by
-  simp only [generateSeedFrom, bind_pure_comp, List.foldlM_cons, bind_map_left]
+  simp [generateSeedFrom]
 
 /-- Taking `n` elements after dropping `l1.length` from `l1 ++ l2 ++ l3` returns `l2`
 if `l2.length = n`. -/
 lemma List.take_drop_append_of_length_eq {α} (l1 l2 l3 : List α) (n : ℕ) (h : l2.length = n) :
-    ((l1 ++ l2 ++ l3).drop l1.length).take n = l2 := by
-  simp [h]
+    ((l1 ++ l2 ++ l3).drop l1.length).take n = l2 := by simp [h]
 
 /-- `ForIn.forIn` on a list with a body that always yields is equivalent to `List.foldlM`. -/
 lemma forIn_list_eq_foldlM.{u} {m : Type → Type u} [Monad m] [LawfulMonad m] {α β : Type}
@@ -333,35 +392,32 @@ lemma forIn_list_eq_foldlM.{u} {m : Type → Type u} [Monad m] [LawfulMonad m] {
   simp
 
 /-- `generateSeed` is equivalent to `generateSeedFrom` with empty initial seed. -/
-lemma generateSeed_eq_generateSeedFrom (spec : OracleSpec ι) [∀ i, SelectableType (spec.range i)]
+lemma generateSeed_eq_generateSeedFrom' (spec : OracleSpec ι) [∀ i, SelectableType (spec.range i)]
     (qc : ι → ℕ) (js : List ι) :
     generateSeed spec qc js = generateSeedFrom spec qc js ∅ := by
   convert forIn_list_eq_foldlM ..
-  · simp only [generateSeed, QuerySeed.instEmptyCollection, bind_pure_comp, map_pure,
-      bind_pure, Functor.map_map]
-  · exact instLawfulMonad
+  · simp only [generateSeed, bind_pure_comp, map_pure, Functor.map_map, bind_pure]
+  · infer_instance
 
 /-- The support of `generateSeedFrom` consists of seeds that extend the initial seed by the correct
 number of elements for each index. -/
-lemma support_generateSeedFrom [spec.FiniteRange] (js : List ι) (seed : QuerySeed spec) :
+lemma support_generateSeedFrom' [spec.FiniteRange] (js : List ι) (seed : QuerySeed spec) :
     (generateSeedFrom spec qc js seed).support =
     {s | ∀ i, List.IsPrefix (seed i) (s i) ∧
       (s i).length = (seed i).length + qc i * js.count i} := by
-  induction' js using List.reverseRecOn with js j ih generalizing seed
-  · ext
+  induction js using List.reverseRecOn generalizing seed with
+  | nil =>
+    ext
     simp only [generateSeedFrom, bind_pure_comp, List.foldlM_nil, support_pure,
       Set.mem_singleton_iff, List.count_nil, mul_zero, add_zero, Set.mem_setOf_eq]
     constructor <;> intro h
     · grind
-    · suffices h_eq : ∀ i, seed i = ‹spec.QuerySeed› i by exact (QuerySeed.ext seed _ h_eq).symm
-      intro i; specialize h i; obtain ⟨h₁, h₂⟩ := h
-      exact h₁.eq_of_length h₂.symm
-  · have h_split : generateSeedFrom spec qc (js ++ [j]) seed = do
+    · exact funext fun i ↦ ((h i).1.eq_of_length (h i).2.symm).symm
+  | append_singleton js j ih =>
+    have h_split : generateSeedFrom spec qc (js ++ [j]) seed = do
       let seed' ← generateSeedFrom spec qc js seed
       let vals ← ($ᵗ spec.range j).replicate (qc j)
-      return seed'.addValues vals := by
-        unfold generateSeedFrom
-        simp [List.foldlM_append]
+      return seed'.addValues vals := by unfold generateSeedFrom; simp [List.foldlM_append]
     simp_all only [Set.ext_iff, Set.mem_setOf_eq, bind_pure_comp, support_bind,
       support_map, support_replicate, support_uniformOfFintype, Set.mem_univ, implies_true,
       and_true, List.count_append, Set.mem_iUnion, Set.mem_image, exists_prop]
@@ -376,12 +432,10 @@ lemma support_generateSeedFrom [spec.FiniteRange] (js : List ι) (seed : QuerySe
           if i = j then x i |>.take (List.length (seed i) + qc i * List.count i js) else x i
       · grind
       · refine ⟨x j |>.drop (List.length (seed j) + qc j * List.count j js), ?_, ?_⟩
-        <;> simp_all only [List.nodup_cons, List.not_mem_nil, not_false_eq_true,
-          List.nodup_nil, and_self, List.length_drop, List.mem_cons, or_false,
-          List.count_eq_one_of_mem]
-        · exact Nat.sub_eq_of_eq_add <| by ring
-        · ext i; by_cases hi : i = j <;> simp_all [List.take_append_drop]
-          · subst hi; simp_all only [Function.update_self]
+        · grind
+        · ext i; by_cases hi : i = j
+          · subst hi; simp_all [List.take_append_drop, Function.update_self]
+          · simp_all [List.take_append_drop]
 
 /-- If `seed_out` is a possible result of `generateSeedFrom` starting with `seed_in` extended by
 `vals`, then `vals` can be recovered from `seed_out`. -/
@@ -391,17 +445,16 @@ lemma vals_eq_of_mem_support_generateSeedFrom [spec.FiniteRange]
     (h_len : vals.length = qc j)
     (h_support : seed_out ∈ (generateSeedFrom spec qc js (seed_in.addValues vals)).support) :
     vals = ((seed_out j).drop (seed_in j).length).take (qc j) := by
-  obtain ⟨k, hk⟩ := (support_generateSeedFrom spec qc js (QuerySeed.addValues vals seed_in)
+  obtain ⟨k, hk⟩ := (support_generateSeedFrom' spec qc js (seed_in.addValues vals)
     |>.subset h_support j).1
-  simp_all [← hk]
+  simp [*, ← hk]
 
 omit [(i : ι) → SelectableType (spec.range i)] in
 /-- If `seed` extended by `vals` is a prefix of `seed'`, then `vals` is determined by
 `seed`, `seed'`. -/
 lemma vals_eq_of_isPrefix_addValues {i : ι} {seed seed' : QuerySeed spec}
     {vals : List (spec.range i)}
-    (h : List.IsPrefix ((seed.addValues vals) i) (seed' i))
-    (n : ℕ) (h_len : vals.length = n) :
+    (h : List.IsPrefix ((seed.addValues vals) i) (seed' i)) (n : ℕ) (h_len : vals.length = n) :
     vals = ((seed' i).drop (seed i).length).take n := by
   obtain ⟨l, hl⟩ := h
   simp [← hl, h_len]
@@ -414,7 +467,7 @@ lemma vals_eq_of_mem_support_generateSeedFrom' [spec.FiniteRange]
     (h_len : vals.length = qc j)
     (h_support : seed_out ∈ (generateSeedFrom spec qc js (seed_in.addValues vals)).support) :
     vals = ((seed_out j).drop (seed_in j).length).take (qc j) :=
-  vals_eq_of_mem_support_generateSeedFrom spec qc js seed_in seed_out j vals h_len h_support
+  vals_eq_of_mem_support_generateSeedFrom _ _ _ _ _ _ _ h_len h_support
 
 omit [DecidableEq ι] in
 /-- Probability of a list from replicating a uniform distribution. -/
@@ -427,7 +480,7 @@ lemma probOutput_replicate_uniformOfFintype [spec.FiniteRange] (j : ι) (n : ℕ
 
 /-- The probability of a specific seed in `generateSeedFrom` is the inverse of the product of the
 cardinalities of the ranges. -/
-lemma probOutput_generateSeedFrom [spec.FiniteRange] [DecidableEq spec.QuerySeed]
+lemma probOutput_generateSeedFrom' [spec.FiniteRange] [DecidableEq spec.QuerySeed]
     (js : List ι) (seed_in : QuerySeed spec) (seed_out : QuerySeed spec)
     (h : seed_out ∈ (generateSeedFrom spec qc js seed_in).support) :
     [= seed_out | generateSeedFrom spec qc js seed_in] =
@@ -437,49 +490,85 @@ lemma probOutput_generateSeedFrom [spec.FiniteRange] [DecidableEq spec.QuerySeed
       Set.mem_singleton_iff, probOutput_pure, ↓reduceIte, List.map_nil, List.prod_nil,
       Nat.cast_one, inv_one]
   | cons j js ih =>
-    have h_def : generateSeedFrom spec qc (j :: js) seed_in =
-        (($ᵗ spec.range j).replicate (qc j) >>= fun vals ↦
-          generateSeedFrom spec qc js (seed_in.addValues vals)) :=
-      generateSeedFrom_cons spec qc j js seed_in
-    have h_bind : [=seed_out|generateSeedFrom spec qc (j :: js) seed_in] =
-        ∑' (vals : List (spec.range j)), [=vals|($ᵗ spec.range j).replicate (qc j)] *
-          [=seed_out|generateSeedFrom spec qc js (seed_in.addValues vals)] := by
-      rw [h_def]
-      exact probOutput_bind_eq_tsum (replicate (qc j) ($ᵗspec.range j))
-        (fun vals ↦ generateSeedFrom spec qc js (QuerySeed.addValues vals seed_in)) seed_out
+    have h_bind : [= seed_out | generateSeedFrom spec qc (j :: js) seed_in] =
+        ∑' (vals : List (spec.range j)), [= vals | ($ᵗ spec.range j).replicate (qc j)] *
+          [= seed_out | generateSeedFrom spec qc js (seed_in.addValues vals)] :=
+      (generateSeedFrom_cons spec qc j js seed_in) ▸
+        probOutput_bind_eq_tsum (replicate (qc j) ($ᵗ spec.range j))
+          (fun vals ↦ generateSeedFrom spec qc js (QuerySeed.addValues vals seed_in)) seed_out
     obtain ⟨vals, h_vals⟩ : ∃ vals : List (spec.range j),
         vals.length = qc j ∧
           seed_out ∈ (generateSeedFrom spec qc js (seed_in.addValues vals)).support := by
       contrapose! h_bind
-      simp_all
+      simp_all [generateSeedFrom_cons]
     rw [h_bind, tsum_eq_single vals]
     · rw [probOutput_replicate_uniformOfFintype, if_pos h_vals.1, ih _ _ h_vals.2]
       simp only [Nat.cast_list_prod, List.map_map, List.map_cons, List.prod_cons,
         Nat.cast_mul, Nat.cast_pow]
       rw [ENNReal.mul_inv]
-      · left
-        exact ENNReal.pow_ne_zero (Nat.cast_ne_zero.mpr Fintype.card_pos.ne') _
-      · left
-        exact ENNReal.pow_ne_top ENNReal.coe_ne_top
+      · exact .inl (ENNReal.pow_ne_zero (Nat.cast_ne_zero.mpr Fintype.card_pos.ne') _)
+      · exact .inl (ENNReal.pow_ne_top ENNReal.coe_ne_top)
     · intro b' hb'
       by_cases hb'_len : b'.length = qc j
-      · by_cases hb'_support :
-            seed_out ∈ (generateSeedFrom spec qc js (seed_in.addValues b')).support
-        · have hb'_eq := vals_eq_of_mem_support_generateSeedFrom' spec qc js seed_in seed_out j b'
-            hb'_len hb'_support
-          have hvals_eq := vals_eq_of_mem_support_generateSeedFrom' spec qc js seed_in seed_out j
-            vals h_vals.1 h_vals.2
-          exact (hb' (hb'_eq.trans hvals_eq.symm)).elim
-        · exact mul_eq_zero_of_right _ (by rw [probOutput_eq_zero_iff]; grind)
+      · refine mul_eq_zero_of_right _ ?_
+        rw [probOutput_eq_zero_iff]
+        intro hb'_support
+        exact hb' ((vals_eq_of_mem_support_generateSeedFrom' spec qc js seed_in seed_out j b'
+            hb'_len hb'_support).trans
+          (vals_eq_of_mem_support_generateSeedFrom' spec qc js seed_in seed_out j
+            vals h_vals.1 h_vals.2).symm)
       · rw [probOutput_replicate_uniformOfFintype, if_neg hb'_len, zero_mul]
 
 lemma probOutput_generateSeed' [spec.FiniteRange]
     [DecidableEq spec.QuerySeed] (seed : QuerySeed spec)
     (h : seed ∈ (generateSeed spec qc js).support) : [= seed | generateSeed spec qc js] =
     ((generateSeed spec qc js).finSupport.card : ℝ≥0∞)⁻¹ := by
-  convert probOutput_generateSeedFrom spec qc js ∅ seed _ using 1
-  · rw [generateSeed_eq_generateSeedFrom]
-  · rw [card_finSupport_generateSeed]
-  · exact generateSeed_eq_generateSeedFrom spec qc js ▸ h
+  rw [card_finSupport_generateSeed, generateSeed_eq_generateSeedFrom]
+  exact probOutput_generateSeedFrom' spec qc js ∅ seed <|
+    generateSeed_eq_generateSeedFrom' spec qc js ▸ h
+
+-- sorry
+--   revert seed
+--   induction js with
+--   | nil => {
+--     intro seed h
+--     simp at h
+--     simp [h]
+--   }
+--   | cons j js hjs => {
+--     intro seed h
+--     let rec_seed : QuerySeed spec := seed.takeAtIndex j (qc j * js.count j)
+--     specialize hjs rec_seed _
+--     · simp [rec_seed]
+--       rw [support_generateSeed, Set.mem_setOf] at h
+--       intro k
+--       by_cases hk : k = j
+--       · induction hk
+--         let hk := h k
+--         rw [List.count_cons_self, mul_add_one] at hk
+--         simp [rec_seed, QuerySeed.takeAtIndex, hk]
+--       · simp [rec_seed, QuerySeed.takeAtIndex, hk, h k]
+--     · rw [generateSeed_cons]
+--       have : seed = QuerySeed.addValues rec_seed ((seed j).drop <| qc j * js.count j) :=
+--         funext (λ k ↦ by simp [rec_seed, QuerySeed.takeAtIndex, QuerySeed.addValues])
+--       refine (probOutput_seq_map_eq_mul _ _ QuerySeed.addValues rec_seed
+--         (((seed j).drop <| qc j * js.count j)) _ ?_).trans ?_
+--       · simp
+--         intro seed' hs' xs
+--         simp [rec_seed]
+--         rw [QuerySeed.eq_addValues_iff]
+--         simp [hs']
+--       · rw [hjs]
+--         rw [support_generateSeed, Set.mem_setOf] at h
+--         specialize h j
+--         simp only [List.count_cons_self] at h
+--         simp only [Nat.cast_list_prod, List.map_map, one_div, probOutput_vector_toList,
+--           List.length_drop, h, mul_add_one, add_tsub_cancel_left, ↓reduceDIte,
+              -- probOutput_replicate,
+--           probOutput_uniformOfFintype, Vector.toList_mk, List.map_drop, List.map_const',
+--           List.drop_replicate, List.prod_replicate, List.map_cons, List.prod_cons, Nat.cast_mul,
+--           Nat.cast_pow]
+--         rw [mul_comm, ← ENNReal.inv_pow, ENNReal.mul_inv] <;> simp
+--   }
 
 end OracleComp
